\documentclass{article}
\usepackage[letterpaper, margin=0.05in]{geometry}
\usepackage{multicol}
\usepackage{graphicx}
\usepackage{amsmath}
\usepackage{array}
\usepackage{xcolor,colortbl}


\begin{document}
\large
\section{Definition}
$a^x = b \Leftrightarrow \log_ab = x$

\section{Zero Rule}
\begin{multicols}{2}
    $\log(1) = 0$\\ $\ln(1) = 0$
\end{multicols}

\section{log of the same number as base}
\begin{multicols}{2}
    $\log_a(a) = 1$ \\ $\ln(e) = 1$
\end{multicols}

\section{Product Rule}
\begin{multicols}{2}
    $\log_a(xy) = \log_a(x) + \log_a(y)$ \\ $\ln(xy) = \ln(x) + \ln(y)$
\end{multicols}

\section{Quotient Rule}
\begin{multicols}{2}
    $\log_a\left(\dfrac{x}{y}\right) = \log_a(x) - \log_a(y)$ \\ $\ln\left(\dfrac{x}{y}\right) = \ln(x) + \ln(y)$
\end{multicols}

\section{Power Rule}
\begin{multicols}{2}
    $\log_a(x^y) = y\log_a(x)$ \\ $\ln(x^y) = y\ln(x)$
\end{multicols}

\section{Change of base Rule}
\begin{multicols}{2}
    $\log_a(x) = \dfrac{\log_b(x)}{\log_b(y)}$ \\ $\log_a(x) \cdot \log_b(y) = \log_c(y)$
\end{multicols}

\section{Equality Rule}
\begin{multicols}{2}
    $\log_a(x) = \log_a(y) \Rightarrow x=y$ \\ $\ln(x) = \ln(y) \Rightarrow x = y$
\end{multicols}

\section{Number Raised to Log}
\begin{multicols}{2}
    $b^{\log_bx} = x$ \\ $e^{\ln x} = x$
\end{multicols}

\section{Others}
\begin{multicols}{2}
    $-\log_ax=\log_a \left(\dfrac{1}{x}\right)$
\end{multicols}

\end{document}